hardware/ag32MachineScript.sml
@@ -49,6 +49,9 @@ val _ = Datatype `
                 acc_state : word2
               |>`;
 
+val _ = Datatype `
+ interrupt_state = InterruptReady | InterruptWorking | InterruptAck`;
+
 (* External inputs, and model of relevant part of world (i.e., contents of memory) *)
 val _ = Datatype `
  ext = <| (* in state_circuit for now, but "should" be here...
@@ -67,7 +70,9 @@ val _ = Datatype `
           mem_start_input : word32;
 
           (* Interrupt *)
-          interrupt_ack : bool
+          interrupt_state : interrupt_state;
+          interrupt_ack : bool;
+          io_events : (word32 -> word32) list
         |>`;
 
 (** Memory specification **)
@@ -152,12 +157,30 @@ val is_mem_start_interface_def = Define `
   ?n. (!m. m < n ==> ~(fext m).mem_start_ready) /\ (fext n).mem_start_ready /\ (fext n).mem_start_input = mem_start`;
 
 (** Interrupt interface **)
-(* Very weak specification, could make the it more detailed. Can e.g. not prove absence of spurious acks using this.
-   Also not entirely sound model, because in reality stacking of interrupts is not possible
-   (and must ack each interrupt requested, otherwise host core waits forever). *)
+
+(* This is a little difficult to model properly because the interrupt interface is async. *)
 val is_interrupt_interface_def = Define `
  is_interrupt_interface circuit fext =
-  !n. (circuit n).interrupt_req ==> ?m. (fext (SUC (n + m))).interrupt_ack`;
+  ((fext 0).io_events = [] /\
+  (fext 0).interrupt_state = InterruptReady /\
+  !n. case (fext n).interrupt_state of
+         InterruptReady =>
+          if (circuit n).interrupt_req then
+           ?m. (!p. p < m ==> ~(fext (SUC (n + p))).interrupt_ack) /\
+               (fext (SUC (n + m))).interrupt_state = InterruptAck /\
+               (* This assumes that memory is not changed during interrupts,
+                  this assumption could be added as a precondition. *)
+               (fext (SUC (n + m))).io_events = (fext n).mem :: (fext n).io_events /\
+               (fext (SUC (n + m))).interrupt_ack
+          else
+           (fext (SUC n)).interrupt_state = InterruptReady /\
+           (fext (SUC n)).io_events = (fext n).io_events /\
+           ~(fext (SUC n)).interrupt_ack
+       | InterruptWorking => T
+       | InterruptAck =>
+         (fext (SUC n)).interrupt_state = InterruptReady /\
+         (fext (SUC n)).io_events = (fext n).io_events /\
+         ~(fext (SUC n)).interrupt_ack)`;
 
 (** Cpu implementation **)
 
